Fixed up chaining

10ChainedEnvironment/ChainedEnvironment.thy
@@ -9,14 +9,15 @@ datatype ceclosure =
 datatype chained_state = 
   CES "ceclosure heap" "(ptr \<times> ptr) heap" "ptr list" "(ptr \<times> nat) list"
 
-primrec chain_lookup :: "('a \<times> ptr) heap \<Rightarrow> ptr \<Rightarrow> nat \<Rightarrow> 'a" where
-  "chain_lookup h p 0 = (case hlookup h p of (a, b) \<Rightarrow> a)"
-| "chain_lookup h p (Suc x) = chain_lookup h (case hlookup h p of (a, b) \<Rightarrow> b) x"
+fun chain_lookup :: "('a \<times> ptr) heap \<Rightarrow> ptr \<Rightarrow> nat \<rightharpoonup> 'a" where
+  "chain_lookup h 0 x = None"
+| "chain_lookup h (Suc p) 0 = Some (case hlookup h p of (a, b) \<Rightarrow> a)"
+| "chain_lookup h (Suc p) (Suc x) = chain_lookup h (case hlookup h p of (a, b) \<Rightarrow> b) x"
 
 inductive evalce :: "byte_code list \<Rightarrow> chained_state \<Rightarrow> chained_state \<Rightarrow> bool" 
     (infix "\<tturnstile> _ \<leadsto>\<^sub>c\<^sub>e" 50) where
-  evce_lookup [simp]: "cd ! pc = BLookup x \<Longrightarrow> 
-    cd \<tturnstile> CES h env vs ((p, Suc pc) # sfs) \<leadsto>\<^sub>c\<^sub>e CES h env (chain_lookup env p x # vs) ((p, pc) # sfs)"
+  evce_lookup [simp]: "cd ! pc = BLookup x \<Longrightarrow> chain_lookup env p x = Some v \<Longrightarrow>
+    cd \<tturnstile> CES h env vs ((p, Suc pc) # sfs) \<leadsto>\<^sub>c\<^sub>e CES h env (v # vs) ((p, pc) # sfs)"
 | evce_pushcon [simp]: "cd ! pc = BPushCon k \<Longrightarrow> halloc h (CEConst k) = (h', v) \<Longrightarrow>
     cd \<tturnstile> CES h env vs ((p, Suc pc) # sfs) \<leadsto>\<^sub>c\<^sub>e CES h' env (v # vs) ((p, pc) # sfs)"
 | evce_pushlam [simp]: "cd ! pc = BPushLam pc' \<Longrightarrow> 
@@ -25,17 +26,17 @@ inductive evalce :: "byte_code list \<Rightarrow> chained_state \<Rightarrow> ch
 | evce_apply [simp]: "cd ! pc = BApply \<Longrightarrow> hlookup h v2 = CELam p' pc' \<Longrightarrow>
     halloc env (v1, p') = (env', p'') \<Longrightarrow> 
       cd \<tturnstile> CES h env (v1 # v2 # vs) ((p, Suc pc) # sfs) \<leadsto>\<^sub>c\<^sub>e 
-        CES h env' vs ((p'', pc') # (p, pc) # sfs)"
+        CES h env' vs ((Suc p'', pc') # (p, pc) # sfs)"
 | evce_return [simp]: "cd ! pc = BReturn \<Longrightarrow> 
     cd \<tturnstile> CES h env vs ((p, Suc pc) # sfs) \<leadsto>\<^sub>c\<^sub>e CES h env vs sfs"
 | evce_jump [simp]: "cd ! pc = BJump \<Longrightarrow> hlookup h v2 = CELam p' pc' \<Longrightarrow>
     halloc env (v1, p') = (env', p'') \<Longrightarrow>
-      cd \<tturnstile> CES h env (v1 # v2 # vs) ((p, Suc pc) # sfs) \<leadsto>\<^sub>c\<^sub>e CES h env' vs ((p'', pc') # sfs)"
+      cd \<tturnstile> CES h env (v1 # v2 # vs) ((p, Suc pc) # sfs) \<leadsto>\<^sub>c\<^sub>e CES h env' vs ((Suc p'', pc') # sfs)"
 
 theorem determinismh: "cd \<tturnstile> \<Sigma> \<leadsto>\<^sub>c\<^sub>e \<Sigma>' \<Longrightarrow> cd \<tturnstile> \<Sigma> \<leadsto>\<^sub>c\<^sub>e \<Sigma>'' \<Longrightarrow> \<Sigma>' = \<Sigma>''"
 proof (induction \<Sigma> \<Sigma>' rule: evalce.induct)
-  case (evce_lookup cd pc x h env vs p sfs)
-  from evce_lookup(2, 1) show ?case 
+  case (evce_lookup cd pc x env p v h vs sfs)
+  from evce_lookup(3, 1, 2) show ?case 
     by (induction cd "CES h env vs ((p, Suc pc) # sfs)" \<Sigma>'' rule: evalce.induct) simp_all 
 next
   case (evce_pushcon cd pc k h h' v env vs p sfs)
